\documentclass[10pt]{article}
\usepackage{fullpage}
\usepackage[utf8]{inputenc}
\usepackage{url}
\usepackage{graphicx}
%\renewcommand{\labelenumi}{(\alph{enumi})}
%\renewcommand{\labelenumii}{(\roman{enumii})}
\renewcommand{\labelenumi}{(\roman{enumi})}

\input macros

\begin{document}

\noindent TA: Ondřej Čertík\\
web: \url{http://hpfem.math.unr.edu/~ondrej/}\\
class: MATH 181\\
date: February 24, 2009

\section*{Quiz 11}

\subsection*{Problem 1}

Page 198, problem 16.
$$z(w) =   w ^ {3/2} (w + c e^w)$$

\subsection*{Problem 2}

Page 198, problem 16.
$$f(x) = {1-xe^x\over x+e^x}$$

\subsection*{Solution to the Problem 1}

$$z'(w) = (w^{3/2} w + w^{3/2}ce^w)'=(w^{5/2}+w^{3/2}ce^w)'
={5\over2}w^{3/2}+{3\over2}w^{1\over2} c e^w + w^{3/2}ce^w$$

\subsection*{Solution to the Problem 2}

$$f'(x) = {(1-xe^x)'(x+e^x)-(1-xe^x)(x+e^x)'\over(x+e^x)^2}
={-(e^x+xe^x)(x+e^x)-(1-xe^x)(1+e^x)\over(x+e^x)^2}=
$$
$$
={-(xe^x+e^{2x}+x^2e^x+xe^{2x})-(1+e^x-xe^x-xe^{2x})\over(x+e^x)^2}
={-xe^x-e^{2x}-x^2e^x-xe^{2x}-1-e^x+xe^x+xe^{2x}\over(x+e^x)^2}
$$
$$
={-e^{2x}-x^2e^x-1-e^x\over(x+e^x)^2}
$$

\end{document}
